# Evaluation

```haskell
add 0 m = m
add n m = inc (add (dec n) m)

add' 0 m = m
add' n m = add' (dec n) (inc m)

inc n = n + 1
dec n = n â€“ 1
```

## Call-By-Need

### (add 2 3)

```haskell
> add (2 3)
= inc (add (dec 2) 3)
= {(add (dec 2) 3)} + 1
= (add (2-1) 3) + 1
= (add 1 3) + 1
= (inc (add (dec 1) 3)) + 1
```

## Call-By-Name

### (add 2 3)

```haskell
> (add 2 3)
= inc (add (dec 2) 3)
= (add (dec 2) 3) + 1
= (add (2-1) 3) + 1
= (add 1 3) + 1
= ((add (dec 1) 3) + 1) + 1
= ((add (1-1) 3) + 1) + 1
= ((add 0 3) + 1) + 1
= (3 + 1) + 1
= 4 + 1
= 5
```

### (add' 2 3)

```haskell
> (add' 2 3)
= add' (dec 2) (inc 3)
= add' (2-1) (inc 3)
= add' 1 (inc 3)
= add' (dec 1) (inc (inc 3))
= add' (1-1) (inc (inc 3))
= add' 0 (inc (inc 3))
= inc (inc 3)
= (inc 3) + 1
= (3+1) + 1
= 4 + 1
= 5
```

## Call-By-Value

### (add 2 3)

```haskell
> (add 2 3)
= inc (add (dec 2) 3)
= inc (add (2-1) 3)
= inc (add 1 3)
= inc (inc (add (dec 1) 3))
= inc (inc (add (1-1) 3))
= inc (inc (add 0 3))
= inc (inc 3)
= inc (3+1)
= inc 4
= 4+1
= 5
```

### (add' 2 3)

```haskell
> (add' 2 3)
= add' (dec 2) (inc 3)
= add' (2-1) (inc 3)
= add' 1 (inc 3)
= add' 1 (3+1)
= add' 1 4
= add' (dec 1) (inc 4)
= add' (1-1) (inc 4)
= add' 0 (inc 4)
= add' 0 (4+1)
= add' 0 5
= 5
```
